Tried to replace reveal by showing the property with pkenc_input but failed

src/lib/communication/DY.Lib.Communication.Core.Lemmas.fst
@@ -17,24 +17,40 @@ open DY.Lib.Communication.Core.Invariants
 
 (**** Confidential Send and Receive Lemmas ****)
 
+#push-options "--fuel 0 --ifuel 1 --z3rlimit 50"
 val encrypt_message_proof:
   {|cinvs:crypto_invariants|} ->
   tr:trace ->
   sender:principal -> receiver:principal -> 
-  pk_receiver:bytes -> nonce:bytes -> payload:bytes ->
+  pk_receiver:bytes -> nonce:bytes -> pkenc_in:pkenc_input ->
   Lemma
   (requires
-    has_communication_layer_crypto_predicates /\
+    has_communication_layer_invariants /\
     is_secret (long_term_key_label sender) tr nonce /\
     nonce `has_usage tr` PkNonce /\
     is_public_key_for tr pk_receiver (LongTermPkEncKey comm_layer_pkenc_tag) receiver /\
-    is_knowable_by (join (principal_label sender) (principal_label receiver)) tr payload /\
-    event_triggered tr sender (CommConfSendMsg sender receiver payload)
+    (
+      match pkenc_in with
+      | PkEncInput payload -> (
+        is_knowable_by (join (principal_label sender) (principal_label receiver)) tr payload /\
+        event_triggered tr sender (CommConfSendMsg sender receiver payload)
+      )
+      | PkEncSignInput {sender=sender'; receiver=receiver'; payload} -> (
+        sender == sender' /\
+        receiver == receiver' /\
+        is_knowable_by (join (principal_label sender) (principal_label receiver)) tr payload /\
+        event_triggered tr sender (CommConfSendMsg sender receiver payload) /\
+        event_triggered tr sender (CommConfAuthSendMsg sender receiver payload)
+      )
+    )
   )
   (ensures
-    is_publishable tr (encrypt_message pk_receiver nonce payload)
+    is_publishable tr (encrypt_message pk_receiver nonce pkenc_in)
   )
-let encrypt_message_proof #cinvs tr sender receiver pk_receiver nonce payload = ()
+let encrypt_message_proof #cinvs tr sender receiver pk_receiver nonce pkenc_in =
+  serialize_wf_lemma pkenc_input (is_knowable_by (join (principal_label sender) (principal_label receiver)) tr) pkenc_in;
+  ()
+#pop-options
 
 val send_confidential_proof:
   {|invs:protocol_invariants|} ->
@@ -64,20 +80,19 @@ let send_confidential_proof #invs tr higher_layer_preds keys_sess_ids sender rec
   match send_confidential keys_sess_ids sender receiver payload tr with
   | (None, tr_out) -> ()
   | (Some _, tr_out) -> (
-    let (Some pk_receiver, tr') = get_public_key sender keys_sess_ids.pki (LongTermPkEncKey comm_layer_pkenc_tag) receiver tr in
-    let (nonce, tr') = mk_rand PkNonce (long_term_key_label sender) 32 tr' in
-    higher_layer_preds.send_conf_later tr tr' sender receiver payload;
-    let ((), tr') = trigger_event sender (CommConfSendMsg sender receiver payload) tr' in
-    assert(event_triggered tr' sender (CommConfSendMsg sender receiver payload));
-    encrypt_message_proof tr' sender receiver pk_receiver nonce payload;
-    let msg_encrypted = encrypt_message pk_receiver nonce payload in
-    let (msg_id, tr') = send_msg msg_encrypted tr' in
-    assert(tr_out == tr');
-    assert(trace_invariant tr_out);
+    let (Some pk_receiver, tr) = get_public_key sender keys_sess_ids.pki (LongTermPkEncKey comm_layer_pkenc_tag) receiver tr in
+    let (nonce, tr) = mk_rand PkNonce (long_term_key_label sender) 32 tr in
+    let ((), tr) = trigger_event sender (CommConfSendMsg sender receiver payload) tr in
+    let msg_encrypted = encrypt_message pk_receiver nonce (PkEncInput payload) in
+    assert(higher_layer_preds.send_conf sender receiver payload tr);
+    assert(event_triggered tr sender (CommConfSendMsg sender receiver payload));
+    encrypt_message_proof tr sender receiver pk_receiver nonce (PkEncInput payload);
+    let (msg_id, tr) = send_msg msg_encrypted tr in
+    assert(tr_out == tr);
     ()
   )
 
-
+#push-options "--fuel 0 --ifuel 2"
 val decrypt_message_proof:
   {|cinvs:crypto_invariants|} ->
   tr:trace ->
@@ -90,7 +105,7 @@ val decrypt_message_proof:
   )
   (ensures (
     match decrypt_message sk_receiver msg_encrypted with
-    | Some payload -> (
+    | Some (PkEncInput payload) -> (
       exists sender. (
         is_knowable_by (join (principal_label sender) (principal_label receiver)) tr payload /\
         (
@@ -99,12 +114,27 @@ val decrypt_message_proof:
         )
       )
     )
+    | Some (PkEncSignInput {sender; receiver; payload}) -> (
+      is_knowable_by (join (principal_label sender) (principal_label receiver)) tr payload /\
+      (
+        (event_triggered tr sender (CommConfSendMsg sender receiver payload) /\
+        event_triggered tr sender (CommConfAuthSendMsg sender receiver payload)
+        ) \/
+        is_publishable tr payload
+      )
+    )
     | _ -> True
   ))
 let decrypt_message_proof #cinvs tr receiver sk_receiver msg_encrypted =
   match decrypt_message sk_receiver msg_encrypted with
-  | Some payload -> ()
-  | _ -> ()
+  | None -> ()
+  | Some pkenc_in -> (
+    let Some plain_payload = pk_dec sk_receiver msg_encrypted in
+    FStar.Classical.move_requires (parse_wf_lemma pkenc_input (is_publishable tr)) plain_payload;
+    parse_wf_lemma pkenc_input (bytes_invariant tr) plain_payload;   
+    ()
+  )
+#pop-options
 
 val receive_confidential_proof:
   {|invs:protocol_invariants|} ->
@@ -157,10 +187,18 @@ val sign_message_proof:
     is_private_key_for tr sk_sender (LongTermSigKey comm_layer_sign_tag) sender /\
     (
       if is_encrypted then (
-        match pk_enc_extract_msg payload with
-        | None -> False
-        | Some plain_payload -> (     
-          event_triggered tr sender (CommConfAuthSendMsg sender receiver plain_payload)
+        (exists (plain_msg:communication_message) nonce pk_receiver.
+          //pk_enc_extract_pk payload == Some (DY.Core.Bytes.Type.Pk sk_receiver) /\
+          //Some plain_msg == pk_dec sk_receiver payload /\
+          payload == encrypt_message pk_receiver nonce (PkEncSignInput plain_msg) /\
+          plain_msg.sender == sender /\
+          bytes_well_formed tr pk_receiver /\
+          pk_receiver `has_sk_usage tr` (long_term_key_type_to_usage (LongTermPkEncKey comm_layer_pkenc_tag) plain_msg.receiver) /\
+          //get_label sk_receiver == principal_label receiver /\
+          //event_triggered tr sender (CommConfSendMsg sender receiver plain_msg) /\
+          //event_triggered tr sender (CommAuthSendMsg sender plain_msg) /\ 
+          event_triggered tr plain_msg.sender (CommConfAuthSendMsg plain_msg.sender plain_msg.receiver plain_msg.payload) //\   
+          //get_label tr plain_msg.payload `can_flow tr` (join (principal_label plain_msg.sender) (principal_label plain_msg.receiver))
         )
       ) else (
         event_triggered tr sender (CommAuthSendMsg sender payload)
@@ -172,11 +210,11 @@ val sign_message_proof:
   )
 let sign_message_proof #cinvs tr sender receiver payload is_encrypted sk_sender nonce =
   if is_encrypted then (
-    let sig_input = Encrypted {sender; receiver; payload} in
+    let sig_input = Encrypted payload in
     let sig_input_bytes = serialize signature_input sig_input in
     serialize_wf_lemma signature_input (is_publishable tr) sig_input;
     let signature = sign sk_sender nonce sig_input_bytes in
-    let msg_signed = {sender; receiver; payload; signature} in
+    let msg_signed = {payload=sig_input_bytes; signature} in
     assert(bytes_invariant tr signature);
     serialize_wf_lemma communication_message_sign (is_publishable tr) msg_signed;
     ()
@@ -185,8 +223,7 @@ let sign_message_proof #cinvs tr sender receiver payload is_encrypted sk_sender 
     let sig_input_bytes = serialize signature_input sig_input in
     serialize_wf_lemma signature_input (is_publishable tr) sig_input;
     let signature = sign sk_sender nonce sig_input_bytes in
-    let msg_signed = {sender; receiver; payload; signature} in
-    assert(bytes_invariant tr signature);
+    let msg_signed = {payload=sig_input_bytes; signature} in
     serialize_wf_lemma communication_message_sign (is_publishable tr) msg_signed;
     ()
   )
@@ -227,7 +264,7 @@ let send_authenticated_proof #invs tr higher_layer_preds comm_keys_ids sender re
       ()
     )
 
-
+#push-options "--fuel 0 --ifuel 1 --z3rlimit 10"
 val verify_message_proof:
   {|cinvs:crypto_invariants|} ->
   tr:trace ->
@@ -242,22 +279,42 @@ val verify_message_proof:
   )
   (ensures (
     match verify_message receiver msg_bytes is_encrypted vk_sender with
-    | Some {sender=sender'; receiver=receiver'; payload} -> (
+    | Some payload -> (
       is_publishable tr payload /\
       (
         (
-          sender' == sender /\
-          (
+          let Some msg_signed = parse communication_message_sign msg_bytes in
+          let Some sign_input = parse signature_input msg_signed.payload in
+          match sign_input with
+          | Plain {sender=sender'; receiver=receiver'; payload=payload'} -> (
+            sender == sender' /\
+            receiver == receiver' /\
+            is_publishable tr payload' /\
+            event_triggered tr sender (CommAuthSendMsg sender payload)
+          )
+          | Encrypted payload -> (
+            exists (plain_payload:communication_message) nonce pk_receiver.
+              payload == encrypt_message pk_receiver nonce (PkEncSignInput plain_payload) /\
+              plain_payload.sender == sender /\
+              bytes_well_formed tr pk_receiver /\
+              pk_receiver `has_sk_usage tr` (long_term_key_type_to_usage (LongTermPkEncKey comm_layer_pkenc_tag) plain_payload.receiver) /\
+              event_triggered tr plain_payload.sender (CommConfAuthSendMsg plain_payload.sender plain_payload.receiver plain_payload.payload)
+          )
+          (*
             if is_encrypted then (
-              match pk_enc_extract_msg payload with
-              | None -> False
-              | Some plain_payload -> (
-                event_triggered tr sender (CommConfAuthSendMsg sender receiver plain_payload)
-              )
+              exists plain_msg nonce pk_receiver.
+                //pk_enc_extract_pk payload == Some (DY.Core.Bytes.Type.Pk sk_receiver) /\
+                //Some plain_msg == decrypt_message sk_receiver payload /\
+                //get_label sk_receiver == principal_label receiver /\
+                payload == encrypt_message pk_receiver nonce plain_msg
+                //event_triggered tr sender (CommConfSendMsg sender receiver plain_msg) /\
+                //event_triggered tr sender (CommAuthSendMsg sender plain_msg) /\
+                //event_triggered tr sender (CommConfAuthSendMsg sender receiver plain_msg) //\
+                //get_label plain_msg `can_flow tr` (join (principal_label sender) (principal_label receiver))
             ) else (
               event_triggered tr sender (CommAuthSendMsg sender payload)
             )
-          )
+          *)
         ) \/ (
           is_corrupt tr (long_term_key_label sender)
         )
@@ -268,21 +325,77 @@ val verify_message_proof:
 let verify_message_proof #cinvs tr sender receiver msg_bytes is_encrypted vk_sender =
   assert(get_signkey_label tr vk_sender == long_term_key_label sender);
   match verify_message receiver msg_bytes is_encrypted vk_sender with
-  | Some {sender=sender'; receiver=receiver'; payload} -> (
+  | Some payload -> (
+    assert(is_publishable tr msg_bytes);
     parse_wf_lemma communication_message_sign (is_publishable tr) msg_bytes;
     let Some msg_signed = parse communication_message_sign msg_bytes in
+    assert(is_publishable tr msg_signed.payload);
+    parse_wf_lemma signature_input (is_publishable tr) msg_signed.payload;
+    let Some sign_input = parse signature_input msg_signed.payload in
+    assert(is_publishable tr payload);
     
-    if is_encrypted then (
-      let sig_input_e = Encrypted {sender=sender'; receiver=msg_signed.receiver; payload=msg_signed.payload} in
-      serialize_wf_lemma signature_input (is_publishable tr) sig_input_e;
-      ()
-    ) else (
-      let sig_input_p = Plain {sender=sender'; receiver=msg_signed.receiver; payload=msg_signed.payload} in
-      serialize_wf_lemma signature_input (is_publishable tr) sig_input_p;
+    //assert(bytes_invariant tr vk_sender);
+    //assert(bytes_invariant tr msg_bytes);
+    //assert(bytes_invariant tr msg_signed.signature);
+    //normalize_term_spec bytes_invariant;
+    //reveal_opaque (`%verify) (verify);
+    
+
+    (*assert(event_triggered tr sender (CommAuthSendMsg sender payload) \/
+      get_signkey_label vk_sender `can_flow tr` public);
+    
+    let DY.Core.Bytes.Type.Sign sk nonce sig_input_bytes = msg_signed.signature in
+    assert(sign_pred.pred tr (Vk sk) sig_input_bytes \/
+      get_signkey_label vk_sender `can_flow tr` public);
+
+    assert(receiver == receiver');
+    assert(sender == sender' \/
+      get_signkey_label vk_sender `can_flow tr` public);*)
+    
+    match sign_input with
+    | Plain {sender=sender'; receiver=receiver'; payload=payload'} -> (
+      //let sig_input_p = Plain {sender=sender'; receiver=msg_signed.receiver; payload=msg_signed.payload} in
+      //let Some sig_input = parse signature_input msg_signed.payload in
+      //FStar.Classical.move_requires (serialize_wf_lemma signature_input (is_publishable tr)) sign_input;
+      assert(payload == payload');
+      assert(event_triggered tr sender (CommAuthSendMsg sender payload) \/
+        is_corrupt tr (long_term_key_label sender));
       ()
     )
+    | Encrypted payload' -> (
+      //let sig_input_e = Encrypted msg_signed.payload in
+      //let sig_input_bytes_e = serialize signature_input #parseable_serializeable_bytes_signature_input sig_input_e in
+      //serialize_wf_lemma signature_input (is_publishable tr) sign_input;
+      assert(bytes_invariant tr msg_signed.signature);
+      
+      assert(
+        (exists plain_msg nonce pk_receiver.
+          payload == encrypt_message pk_receiver nonce plain_msg) \/
+          is_corrupt tr (long_term_key_label sender)
+      );
+
+      //assert(verify vk_sender sig_input_bytes_e msg_signed.signature);      
+      //assert(bytes_invariant tr sig_input_bytes_e);      
+      //bytes_invariant_verify tr vk_sender sig_input_bytes_e msg_signed.signature;
+
+      (*let Some sig_input = parse signature_input sig_input_bytes in
+      assert(Encrypted? sig_input);
+      let sig_input_record = Encrypted?.msg sig_input in
+      assert(sign_pred.pred tr (Vk sk) sig_input_bytes \/
+        get_signkey_label vk_sender `can_flow tr` public);
+      assert(msg_signed.receiver == receiver);
+      let sig_input' = Encrypted {sender=sender'; receiver=msg_signed.receiver; payload=msg_signed.payload} in
+      let sig_input_bytes' = serialize signature_input sig_input' in
+      assert(verify vk_sender sig_input_bytes' msg_signed.signature);
+      assert(sig_input_record.sender == sender \/
+        get_signkey_label vk_sender `can_flow tr` public);
+      assert(event_triggered tr sender (CommConfSendMsg sender receiver msg) \/
+        get_signkey_label (Vk sk) `can_flow tr` public);*)
+      ()
+    )  
   )
   | _ -> ()
+#pop-options
 
 val receive_authenticated_proof:
   {|invs:protocol_invariants|} ->
@@ -344,9 +457,72 @@ val encrypt_and_sign_message_proof:
     is_publishable tr (encrypt_and_sign_message sender receiver payload pk_receiver sk_sender enc_nonce sign_nonce)
   )
 let encrypt_and_sign_message_proof #cinvs tr sender receiver payload pk_receiver sk_sender enc_nonce sign_nonce =
-  encrypt_message_proof #cinvs tr sender receiver pk_receiver enc_nonce payload;
-  let enc_payload = encrypt_message pk_receiver enc_nonce payload in
-  pk_enc_extract_msg_enc_lemma pk_receiver enc_nonce payload enc_payload;
+  let pkenc_in = PkEncSignInput {sender; receiver; payload} in
+  encrypt_message_proof #cinvs tr sender receiver pk_receiver enc_nonce pkenc_in;
+  let enc_payload = encrypt_message pk_receiver enc_nonce pkenc_in in
+  assert(get_label tr sk_sender == long_term_key_label sender);
+  assert(is_publishable tr enc_payload);
+  assert(enc_payload == encrypt_message pk_receiver enc_nonce pkenc_in);
+  assert(event_triggered tr sender (CommConfSendMsg sender receiver payload));
+  assert(event_triggered tr sender (CommAuthSendMsg sender payload));
+  assert(get_label tr payload `can_flow tr` (join (principal_label sender) (principal_label receiver)));
+  //normalize_term_spec pk_dec;
+  //normalize_term_spec pk_enc;
+  //normalize_term_spec get_sk_label;
+  //normalize_term_spec get_sk_usage;
+  //normalize_term_spec pk;
+
+  (*assert(match pk_receiver with
+  | DY.Core.Bytes.Type.Pk sk -> get_usage sk == PkKey comm_layer_pkenc_tag empty
+  | _ -> False);
+  assert(match pk_receiver with
+  | DY.Core.Bytes.Type.Pk sk -> get_label sk == principal_label receiver
+  | _ -> False);
+
+  assert(is_publishable tr enc_payload);
+
+  assert(enc_payload == pk_enc pk_receiver enc_nonce payload);
+
+  
+    
+  eliminate exists sk_receiver. get_label sk_receiver == principal_label receiver
+  returns exists sk_receiver. pk_dec sk_receiver (pk_enc pk_receiver enc_nonce payload) == Some payload
+  with _. (
+    pk_dec_enc sk_receiver enc_nonce payload;
+    assert(
+        pk_dec sk_receiver (pk_enc (pk sk_receiver) enc_nonce payload) == Some payload
+    );
+    assert(Some payload == decrypt_message sk_receiver enc_payload);
+    assert(exists plain_msg.
+      Some plain_msg == decrypt_message sk_receiver enc_payload
+    );
+    assert(exists plain_msg.
+      get_label plain_msg `can_flow tr` (join (principal_label sender) (principal_label receiver)));
+
+    
+
+    assert(has_communication_layer_invariants cinvs /\
+      is_publishable tr enc_payload /\
+      is_secret (principal_label sender) tr sign_nonce /\
+      SigNonce? (get_usage sign_nonce) /\
+      is_signature_key (SigKey comm_layer_sign_tag empty) (principal_label sender) tr sk_sender /\
+      (
+        if true then (
+          (exists sk_receiver plain_msg.
+            Some plain_msg == pk_dec sk_receiver enc_payload /\
+            get_label sk_receiver == principal_label receiver /\
+            event_triggered tr sender (CommConfSendMsg sender receiver plain_msg) /\
+            event_triggered tr sender (CommAuthSendMsg sender plain_msg) /\      
+            get_label plain_msg `can_flow tr` (join (principal_label sender) (principal_label receiver))
+          )
+        ) else (
+          event_triggered tr sender (CommAuthSendMsg sender payload)
+        )
+      ));
+    sign_message_proof tr sender receiver enc_payload true sk_sender sign_nonce;
+    ()
+  );*)
+  
   sign_message_proof tr sender receiver enc_payload true sk_sender sign_nonce;
   ()
 
@@ -399,46 +575,317 @@ let send_confidential_authenticated_proof #invs tr higher_layer_preds comm_keys_
 #pop-options
 
 
+// TODO rename this function
 val verify_and_decrypt_message_proof:
   {|cinvs:crypto_invariants|} ->
   tr:trace ->
-  sender:principal -> receiver:principal -> msg_encrypted_signed:bytes ->
-  sk_receiver:bytes -> vk_sender:bytes ->
+  receiver:principal -> msg_encrypted_signed:bytes ->
+  sk_receiver:bytes ->
   Lemma
   (requires
     has_communication_layer_crypto_predicates /\
     is_publishable tr msg_encrypted_signed /\
-    is_public_key_for tr vk_sender (LongTermSigKey comm_layer_sign_tag) sender /\
     is_private_key_for tr sk_receiver (LongTermPkEncKey comm_layer_pkenc_tag) receiver
   )
   (ensures (
-    match verify_and_decrypt_message receiver msg_encrypted_signed sk_receiver vk_sender with
+    match decrypt_signed_message receiver sk_receiver msg_encrypted_signed with
     | None -> True
-    | Some {sender=sender'; receiver=receiver'; payload} -> (
+    | Some {sender; receiver=receiver'; payload} -> (
       is_knowable_by (principal_label receiver) tr payload /\
       (
         (
-          sender' == sender /\
-          event_triggered tr sender (CommConfAuthSendMsg sender receiver payload)
+          //event_triggered tr sender (CommAuthSendMsg sender payload) /\        
+          event_triggered tr sender (CommConfSendMsg sender receiver payload) /\
+          event_triggered tr sender (CommConfAuthSendMsg sender receiver payload) ///\
+          //is_knowable_by (join (principal_label sender) (principal_label receiver)) tr payload
         ) \/ (
-          is_corrupt tr (long_term_key_label sender)
+          is_publishable tr payload
         )
       )
     )
   ))
-let verify_and_decrypt_message_proof #cinvs tr sender receiver msg_encrypted_signed sk_receiver vk_sender =
-  match verify_and_decrypt_message receiver msg_encrypted_signed sk_receiver vk_sender with
+let verify_and_decrypt_message_proof #cinvs tr receiver msg_encrypted_signed sk_receiver =
+  match decrypt_signed_message receiver sk_receiver msg_encrypted_signed with
   | None -> ()
   | Some {sender=sender'; receiver=receiver'; payload} -> (
+    assert(is_publishable tr msg_encrypted_signed);
+    parse_wf_lemma communication_message_sign (is_publishable tr) msg_encrypted_signed;
+    //parse_wf_lemma communication_message_sign (bytes_invariant tr) msg_encrypted_signed;
+    let Some signed_msg = parse communication_message_sign msg_encrypted_signed in
+    assert(is_publishable tr signed_msg.payload);
+    parse_wf_lemma signature_input (is_publishable tr) signed_msg.payload;
+    let Some signature_in = parse signature_input signed_msg.payload in
+    let enc_payload = Encrypted?.payload signature_in in
+    assert(is_publishable tr enc_payload);
+    decrypt_message_proof tr receiver sk_receiver enc_payload;
+    let Some (PkEncSignInput cm) = decrypt_message sk_receiver enc_payload in
+    assert(bytes_invariant tr cm.payload);
+    assert(cm.receiver == receiver);
+    assert(event_triggered tr cm.sender (CommConfAuthSendMsg cm.sender cm.receiver cm.payload) \/
+      get_label tr cm.payload `can_flow tr` public);
+    ()
+    
+    (*normalize_term_spec pk_dec;
+    normalize_term_spec pk_enc;
     verify_message_proof tr sender receiver msg_encrypted_signed true vk_sender;
     let Some {sender=sender''; receiver=receiver''; payload=enc_payload} = verify_message receiver msg_encrypted_signed true vk_sender in    
     decrypt_message_proof tr receiver sk_receiver enc_payload;
     let Some payload' = decrypt_message sk_receiver enc_payload in
-    pk_enc_extract_msg_dec_lemma sk_receiver enc_payload payload;
+    
+    //assert(pk_enc_extract_pk enc_payload == Some (DY.Core.Bytes.Type.Pk sk_receiver));
+    assert(payload == payload');
+    assert(exists sender.
+      is_knowable_by (join (principal_label sender) (principal_label receiver)) tr payload /\
+      (       
+        event_triggered tr sender (CommConfSendMsg sender receiver payload) \/
+        is_publishable tr payload
+      )
+    );
+    assert(exists sender. is_knowable_by (join (principal_label sender) (principal_label receiver)) tr payload);
+
+    // TODO transfer this property into the event or separate from the event
+    assert(is_knowable_by (principal_label receiver) tr payload);
+      
     ()
+    *)
+    (*introduce ~(is_corrupt tr (principal_label sender)) /\ ~(is_publishable tr payload) ==> event_triggered tr sender (CommConfSendMsg sender receiver payload)
+    with _. (
+      assert(exists payload. event_triggered tr sender (CommConfSendMsg sender receiver payload));
+      eliminate exists plain_msg. event_triggered tr sender (CommConfSendMsg sender receiver plain_msg)
+      returns event_triggered tr sender (CommConfSendMsg sender receiver payload)
+      with _. (
+        assert(
+          event_triggered tr sender (CommAuthSendMsg sender payload) /\
+          is_knowable_by (join (principal_label sender) (principal_label receiver)) tr payload /\
+          event_triggered tr sender (CommConfSendMsg sender receiver payload)
+        );
+        ()
+      )
+    )*)
+    (*reveal_opaque (`%pk_enc) (pk_enc);
+    reveal_opaque (`%pk_dec) (pk_dec);
+    let DY.Core.Bytes.Type.PkEnc pk nonce msg = enc_payload in
+    assert(if_comm_conf_payload sender receiver'' enc_payload tr \/
+      is_corrupt tr (principal_label sender));
+    assert(get_usage sk_receiver == PkKey comm_layer_pkenc_tag empty);
+    assert(Pk sk_receiver == pk);
+    reveal_opaque (`%get_sk_usage) (get_sk_usage);
+    assert(get_sk_usage pk == PkKey comm_layer_pkenc_tag empty);
+    assert(
+      (
+        get_sk_label pk == principal_label receiver'' /\
+        event_triggered tr sender (CommConfSendMsg sender receiver'' msg)
+      ) \/
+        is_corrupt tr (principal_label sender)                                                        
+    );
+    assert(get_label sk_receiver == principal_label receiver);
+    assert(get_sk_label pk == principal_label receiver'' \/
+      is_corrupt tr (principal_label sender));
+    reveal_opaque (`%get_sk_label) (get_sk_label);
+    assert(receiver == receiver'' \/
+      is_corrupt tr (principal_label sender));
+    decrypt_message_proof tr receiver sk_receiver enc_payload;*)
   )
 
-#push-options "--z3rlimit 10"
+#push-options "--fuel 4 --ifuel 4 --z3rlimit 50"
+(*val has_usage_same_key:
+  {|invs:protocol_invariants|} ->
+  tr:trace ->
+  sk_prin:bytes -> pk_prin:bytes ->
+  usg:usage{PkKey? usg} ->
+  Lemma
+  (requires
+    bytes_well_formed tr sk_prin /\
+    bytes_well_formed tr pk_prin /\
+    sk_prin `has_usage tr` usg /\
+    pk_prin `has_sk_usage tr` usg
+  )
+  (ensures
+    pk_prin == pk sk_prin
+  )
+let has_usage_same_key #invs tr sk_prin pk_prin usg = 
+  normalize_term_spec extract_sk;
+  normalize_term_spec pk;
+  ()*)
+
+val combine_lemma:
+  {|invs:protocol_invariants|} ->
+  tr:trace ->
+  sender:principal -> receiver:principal ->
+  payload:bytes -> enc_payload:bytes ->
+  sk_receiver:bytes ->
+  Lemma
+  (requires
+    has_communication_layer_invariants /\
+    is_publishable tr enc_payload /\
+    bytes_invariant tr payload /\
+    (
+      (exists (plain_payload:communication_message) pk_receiver nonce.
+        enc_payload == encrypt_message pk_receiver nonce (PkEncSignInput plain_payload) /\
+        plain_payload.sender == sender /\
+        event_triggered tr sender (CommConfAuthSendMsg sender plain_payload.receiver plain_payload.payload)
+        //(pk sk_receiver) == pk_receiver
+      ) \/
+      is_corrupt tr (long_term_key_label sender)
+    ) /\ (
+      (
+        event_triggered tr sender (CommConfSendMsg sender receiver payload) /\
+        event_triggered tr sender (CommConfAuthSendMsg sender receiver payload)
+      ) \/ (
+        is_publishable tr payload
+      )
+    ) /\ (
+      let sign_input_bytes = serialize signature_input #parseable_serializeable_bytes_signature_input (Encrypted enc_payload) in
+      let signed_msg_bytes = serialize communication_message_sign #parseable_serializeable_bytes_communication_message_sign {payload=sign_input_bytes; signature=empty} in
+      Some {sender; receiver; payload} = decrypt_signed_message receiver sk_receiver signed_msg_bytes
+    )
+  )
+  (ensures
+    event_triggered tr sender (CommConfAuthSendMsg sender receiver payload) \/
+    is_corrupt tr (long_term_key_label sender) 
+  )
+let combine_lemma #invs tr sender receiver payload enc_payload sk_receiver =
+  assert(forall (plain_payload:communication_message).
+    let pkenc_in_bytes = serialize pkenc_input (PkEncSignInput plain_payload) in
+    (pkenc_pred.pred tr (long_term_key_type_to_usage (LongTermPkEncKey comm_layer_pkenc_tag) receiver) pkenc_in_bytes ==>
+      event_triggered tr plain_payload.sender (CommConfAuthSendMsg plain_payload.sender receiver plain_payload.payload))
+  );
+
+  //normalize_term_spec pk;
+  //normalize_term_spec pk_enc;
+  //normalize_term_spec pk_dec;
+  
+  assert(
+    (exists (plain_payload:communication_message) pk_receiver nonce.
+        enc_payload == encrypt_message pk_receiver nonce (PkEncSignInput plain_payload) /\
+        //decrypt_message sk_receiver enc_payload == Some (PkEncSignInput plain_payload) /\
+        plain_payload.sender == sender /\
+        //plain_payload.receiver == receiver /\
+        //plain_payload.payload == payload /\
+        event_triggered tr sender (CommConfAuthSendMsg sender plain_payload.receiver plain_payload.payload)
+        //(pk sk_receiver) == pk_receiver
+      ) \/
+      is_corrupt tr (long_term_key_label sender)
+  );
+
+  introduce (~(is_corrupt tr (long_term_key_label sender))) ==> 
+    (exists (plain_payload:communication_message) pk_receiver nonce. 
+      enc_payload == encrypt_message pk_receiver nonce (PkEncSignInput plain_payload) /\
+      plain_payload.sender == sender /\
+      event_triggered tr sender (CommConfAuthSendMsg sender receiver payload)
+      //(pk sk_receiver) == pk_receiver
+    )
+  with _. (
+    eliminate exists (plain_payload:communication_message) pk_receiver nonce. 
+      enc_payload == encrypt_message pk_receiver nonce (PkEncSignInput plain_payload) /\
+      plain_payload.sender == sender /\
+      event_triggered tr sender (CommConfAuthSendMsg sender plain_payload.receiver plain_payload.payload)
+      //(pk sk_receiver) == pk_receiver
+    returns (event_triggered tr sender (CommConfAuthSendMsg sender receiver payload)
+    )
+    with _. (
+      pk_dec_enc sk_receiver nonce (serialize pkenc_input (PkEncSignInput plain_payload));
+      let pkenc_in_bytes = serialize pkenc_input #parseable_serializeable_bytes_pkenc_input (PkEncSignInput plain_payload) in
+      assert(enc_payload == pk_enc pk_receiver nonce pkenc_in_bytes);
+      (*
+      The following code needs this precondition:
+      is_private_key_for tr sk_receiver (LongTermPkEncKey comm_layer_pkenc_tag) receiver
+
+      assert(sk_receiver `has_usage tr` (long_term_key_type_to_usage (LongTermPkEncKey comm_layer_pkenc_tag) receiver));
+     
+      assert(decrypt_message sk_receiver enc_payload == Some (PkEncSignInput {sender; receiver; payload}));
+      
+      let b = serialize pkenc_input #parseable_serializeable_bytes_pkenc_input (PkEncSignInput {sender; receiver; payload}) in
+      assert(bytes_invariant tr payload);
+      serialize_wf_lemma pkenc_input (bytes_invariant tr) (PkEncSignInput {sender; receiver; payload});
+      assert(bytes_invariant tr b);
+      assert(bytes_invariant tr enc_payload);
+      parse_wf_lemma pkenc_input (bytes_invariant tr) enc_payload;
+      
+      let Some b' = pk_dec sk_receiver enc_payload in
+      assert(parse pkenc_input b' == Some (PkEncSignInput {sender; receiver; payload}));
+      assert(
+        pkenc_pred.pred tr (long_term_key_type_to_usage (LongTermPkEncKey comm_layer_pkenc_tag) receiver) b' \/
+        is_publishable tr b'  
+      );
+      assert(
+        (        
+          event_triggered tr sender (CommConfAuthSendMsg sender receiver payload) /\
+          is_knowable_by (join (principal_label sender) (principal_label receiver)) tr payload
+        ) \/
+        is_publishable tr b'
+      );
+      assert(plain_payload.sender == sender);
+      assert(event_triggered tr sender (CommConfAuthSendMsg sender plain_payload.receiver plain_payload.payload));
+      //assert(plain_payload.payload == payload);*)
+
+      normalize_term_spec pk_dec;
+      normalize_term_spec pk_enc;
+      
+      assert(event_triggered tr sender (CommConfAuthSendMsg sender receiver payload));
+      
+      
+      assert(Some pkenc_in_bytes == pk_dec sk_receiver enc_payload);
+      assert(Some pkenc_in_bytes == pk_dec sk_receiver (pk_enc pk_receiver nonce pkenc_in_bytes));
+      
+      
+      assert(enc_payload == encrypt_message pk_receiver nonce (PkEncSignInput plain_payload));
+      assert(decrypt_message sk_receiver enc_payload == Some (PkEncSignInput plain_payload));
+      
+      assert(plain_payload.sender == sender);
+      assert(plain_payload.receiver == receiver);
+      assert(plain_payload.payload == payload);
+      
+      
+      ()
+    )
+  );
+ ()
+  
+  (*assert(
+    exists payload.
+      Some payload == pk_dec sk_receiver (pk_enc (pk sk_receiver) nonce payload)
+  );
+  assert(
+    (exists (plain_payload:communication_message) pk_receiver.
+      let pkenc_in_bytes = serialize pkenc_input #parseable_serializeable_bytes_pkenc_input (PkEncSignInput plain_payload) in
+
+      (pk sk_receiver) == pk_receiver /\
+
+      //Some pkenc_in_bytes == pk_dec sk_receiver (pk_enc pk_receiver nonce pkenc_in_bytes) ///\
+
+      enc_payload == pk_enc pk_receiver nonce pkenc_in_bytes /\
+      Some pkenc_in_bytes == pk_dec sk_receiver enc_payload //\
+      //decrypt_message sk_receiver enc_payload == Some (PkEncSignInput plain_payload) /\
+      //plain_payload.sender == sender /\
+      //plain_payload.receiver == receiver /\
+      //plain_payload.payload == payload /\
+      //event_triggered tr sender (CommConfAuthSendMsg sender plain_payload.receiver plain_payload.payload)
+    ) \/
+    is_corrupt tr (long_term_key_label sender)
+  );
+
+  
+  assert(Some (PkEncSignInput {sender; receiver; payload}) == decrypt_message sk_receiver enc_payload);
+  let Some plain_payload = pk_dec sk_receiver enc_payload in
+  FStar.Classical.move_requires (parse_wf_lemma pkenc_input (is_publishable tr)) plain_payload;
+  FStar.Classical.move_requires (parse_wf_lemma pkenc_input (bytes_invariant tr)) plain_payload;
+  assert(
+    (pkenc_pred.pred tr (long_term_key_type_to_usage (LongTermPkEncKey comm_layer_pkenc_tag) receiver) plain_payload \/
+      is_publishable tr plain_payload    
+    ) /\
+    (
+      (        
+        event_triggered tr sender (CommConfAuthSendMsg sender receiver payload) /\
+        is_knowable_by (join (principal_label sender) (principal_label receiver)) tr payload
+      ) \/
+      is_publishable tr payload
+    ) /\
+    Some (PkEncSignInput {sender; receiver; payload}) == parse pkenc_input plain_payload
+  );
+
+  ()*)
+
 val receive_confidential_authenticated_proof:
   {|invs:protocol_invariants|} ->
   tr:trace ->
@@ -469,13 +916,19 @@ let receive_confidential_authenticated_proof #invs tr higher_layer_preds comm_ke
   | (None, tr_out) -> ()
   | (Some {sender; receiver=receiver'; payload}, tr_out) -> (
     let (Some msg_encrypted_signed, tr) = recv_msg msg_id tr in
-    let Some sender = get_sender msg_encrypted_signed in
     let (Some sk_receiver, tr) = get_private_key receiver comm_keys_ids.private_keys (LongTermPkEncKey comm_layer_pkenc_tag) tr in
-    let (Some vk_sender, tr) = get_public_key receiver comm_keys_ids.pki (LongTermSigKey comm_layer_sign_tag) sender tr in
-    verify_and_decrypt_message_proof tr sender receiver msg_encrypted_signed sk_receiver vk_sender;
-    let Some msg = verify_and_decrypt_message receiver msg_encrypted_signed sk_receiver vk_sender in
-    let ((), tr) = trigger_event receiver (CommConfAuthReceiveMsg msg.sender receiver msg.payload) tr in
-    assert(event_triggered tr receiver (CommConfAuthReceiveMsg msg.sender receiver msg.payload));
+    verify_and_decrypt_message_proof tr receiver msg_encrypted_signed sk_receiver;
+    let Some cm = decrypt_signed_message receiver sk_receiver msg_encrypted_signed in
+    let (Some vk_sender, tr) = get_public_key receiver comm_keys_ids.pki (LongTermSigKey comm_layer_sign_tag) cm.sender tr in
+    verify_message_proof tr cm.sender receiver msg_encrypted_signed true vk_sender;
+    
+    let Some msg_signed = parse communication_message_sign msg_encrypted_signed in
+    let Some (Encrypted enc_payload) = parse signature_input msg_signed.payload in
+    combine_lemma tr cm.sender receiver cm.payload enc_payload sk_receiver;
+    
+    let Some _ = verify_message receiver msg_encrypted_signed true vk_sender in
+    let ((), tr) = trigger_event receiver (CommConfAuthReceiveMsg cm.sender receiver cm.payload) tr in
+    assert(event_triggered tr receiver (CommConfAuthReceiveMsg cm.sender receiver cm.payload));
     assert(trace_invariant tr);
     assert(tr == tr_out);
     ()
